examples/csl/SL.ConcurrentActions.fst
@@ -11,7 +11,6 @@ let par_wp' #a #b (wpa : st_wp a) (wpb : st_wp b) post m =
            m == (m1 <*> m2)
         /\ par_comp wpa wpb post m1 m2
 
-(* Silly lemma, but allows to handle goals properly *)
 let par_wp'_lemma
   #a #b
   (#wpa : st_wp a)
@@ -20,8 +19,6 @@ let par_wp'_lemma
   (post : post (a * b))
   (_ : squash (m == (m1 <*> m2)))
   (_ : squash (par_comp wpa wpb post m1 m2))
-  //(_ : squash (wpa (fun a m1' -> forall b. post (a, b) m1') m1))
-  //(_ : squash (wpb (fun b m2' -> forall a. post (a, b) m2') m2))
      : Lemma (m == (m1 <*> m2)
                /\ (par_comp wpa wpb post m1 m2)) = ()
 
@@ -32,101 +29,27 @@ assume val par : (#a:Type) -> (#b:Type) ->
                  (#wpa : st_wp a) ->  (#wpb : st_wp b) ->
                  ($f : (unit -> STATE a wpa)) ->
                  ($g : (unit -> STATE b wpb)) ->
-                 STATE (a * b) (par_wp' wpa wpb)
+                 STATE (a * b) (par_wp' wpa wpb) (* big footprint style *)
 
 
 
 (* Locks and operations *)
- // Locks are over a particular reference r.
- // Can we use a list or a set? Non-trivial to make it work. Even a set of addresses causes many blowups.
- // Can we use a heap predicate? Can we automate frame inference then?
+
 assume new type lock : list sref -> (memory -> Type0) -> Type0
-
-(* Does there exist a memory with domain fp such that pred? *)
-let dom_exists (fp:list sref) (pred:memory -> Type0) : Type0 =
-  let rec aux acc fp : Tot Type0 (decreases fp) =
-    match fp with
-    | [] -> pred acc
-    (* this case prevents spurious `emp <*>` which actually matter (the pattern doesn't kick in?) *)
-    (* the pattern was wrong, so not realy needed now, but we might as well keep it I guess *)
-    | [h] ->
-      let ty = dfst h in
-      let r : ref ty = dsnd #Type #ref h in
-      exists (v:ty). pred (acc <*> r |> v)
-    | h :: t -> (* Note, if we match on the sigma pair here, we might prevent reduction *)
-      let ty = dfst h in
-      let r : ref ty = dsnd #Type #ref h in
-      exists (v:ty). aux (acc <*> r |> v) t
-  in aux emp fp
-
-let test (r s : ref int) = dom_exists [tosref s; tosref r] (fun m -> m <*> emp == m)
-
-(* Do all memories with domain fp satisfy pred? *)
-let dom_forall (fp:list sref) (pred:memory -> Type0) : Type0 =
-  let rec aux acc fp : Tot Type0 (decreases fp) =
-    match fp with
-    | [] -> pred acc
-    (* this case prevents spurious `emp <*>` which actually matter (the pattern doesn't kick in?) *)
-    (* the pattern was wrong, so not realy needed now, but we might as well keep it I guess *)
-    | [h] ->
-      let ty = dfst h in
-      let r : ref ty = dsnd #Type #ref h in
-      forall (v:ty). pred (acc <*> r |> v)
-    | h :: t -> (* Note, if we match on the sigma pair here, we might prevent reduction *)
-      let ty = dfst h in
-      let r : ref ty = dsnd #Type #ref h in
-      forall (v:ty). aux (acc <*> r |> v) t
-  in aux emp fp
 
 let mklock_wp (fp:list sref) (inv : memory -> Type0) post m =
   dom_exists fp (fun m' -> mem_eq (m' == m) /\ inv m /\ (forall (l:lock fp inv). post l emp))
-let frame_mklock_wp fp inv = frame_wp (with_fp fp <| mklock_wp fp inv)
 
 assume val mklock : #inv:(memory -> Type0) -> (fp : list sref) ->
-                    STATE (lock fp inv) (frame_mklock_wp fp inv)
+                    ST (lock fp inv) (mklock_wp fp inv) fp
 
 
 let acquire_wp fp inv l post m = m == emp /\ (dom_forall fp (fun m -> inv m ==> post () m))
-let frame_acquire_wp r inv l = frame_wp (with_fp [] <| acquire_wp r inv l)
 assume val acquire : (#fp: list sref) -> (#inv : (memory -> Type0)) -> (l : lock fp inv) ->
-                     STATE unit (frame_acquire_wp fp inv l)
+                     ST unit (acquire_wp fp inv l) []
 
 
 let release_wp fp inv l post m =
   dom_exists fp (fun m' -> mem_eq (m' == m) /\ inv m /\ post () emp)
-let frame_release_wp fp inv l = frame_wp (with_fp fp <| release_wp fp inv l)
 assume val release : (#fp : list sref) -> (#inv : (memory -> Type0)) -> (l : lock fp inv) ->
-                     STATE unit (frame_release_wp fp inv l)
-
-
-// let locking_wp r l wp post m =
-//     wp (fun x m' -> forall v m1. m' == (r |> v <*> m1) ==> post x m1) m
-// 
-// assume val locking : #a:Type -> #b:Type -> #r:(ref a) -> (l : lock r) ->
-//                      (#wp : st_wp b) -> (f : unit -> STATE b wp) ->
-//                   STATE b (frame_locking_wp r l wp)
-
-
-(* A version with explicit heaps *)
-unfold let par_wp'_exp #a #b (wpa : st_wp a) (wpb : st_wp b) (m1 m2 : memory)
-                       (post : post (a * b)) (m : memory) : Type0 =
-           m == (m1 <*> m2)
-        /\ wpa (fun a m1' -> wpb (fun b m2' -> post (a, b) (m1' <*> m2')) m2) m1
-
-let par_wp_exp #a #b (wpa : st_wp a) (wpb : st_wp b) (m1 m2 : memory) : st_wp (a * b) =
-  frame_wp (par_wp'_exp wpa wpb m1 m2)
-
-assume val par_exp : (#a:Type) -> (#b:Type) ->
-                 (#wpa : st_wp a) ->  (#wpb : st_wp b) ->
-                 (m1 : memory) -> (m2 : memory) ->
-                 ($f : (unit -> STATE a wpa)) ->
-                 ($g : (unit -> STATE b wpb)) ->
-                 STATE (a * b) (par_wp_exp #a #b wpa wpb m1 m2)
-
-(* Unframed, explicit variant. Not very user-friendly. *)
-assume val par_exp' : (#a:Type) -> (#b:Type) ->
-                 (#wpa : st_wp a) ->  (#wpb : st_wp b) ->
-                 (m1 : memory) -> (m2 : memory) ->
-                 ($f : (unit -> STATE a wpa)) ->
-                 ($g : (unit -> STATE b wpb)) ->
-                 STATE (a * b) (par_wp'_exp #a #b wpa wpb m1 m2)
+                     ST unit (release_wp fp inv l) fp
