examples/csl/SL.ConcurrentExamples.fst
@@ -3,8 +3,8 @@ module SL.ConcurrentExamples
 open SL.Base
 open SL.AutoTactic
 
-let left  r () : ST int (fun p m -> exists v. m == r |> v /\ p 1 (r |> v)) [tosref r] by (sl_auto ()) = 1
-let right r () : ST int (fun p m -> exists v. m == r |> v /\ p 2 (r |> v)) [tosref r] by (sl_auto ()) = 2
+let left  r () : ST int (fun p m -> exists v. m == r |> v /\ p 1 (r |> v)) [ii r] by (sl_auto ()) = 1
+let right r () : ST int (fun p m -> exists v. m == r |> v /\ p 2 (r |> v)) [ii r] by (sl_auto ()) = 2
 
 let par1 (r:ref int) (s:ref int) : ST int (fun p m -> exists v w. m == (r |> v <*> s |> w) /\ p 3 (r |> v <*> s |> w)) [] by (sl_auto ())
 =
@@ -12,7 +12,7 @@ let par1 (r:ref int) (s:ref int) : ST int (fun p m -> exists v w. m == (r |> v <
   x + y
 
 let par2 (r:ref int) (s:ref int) : ST int (fun p m -> exists v w. m == (r |> v <*> s |> w) /\ p 3 (r |> v <*> s |> w))
-			            [tosref r; tosref s] by (sl_auto ())
+			            [ii r; ii s] by (sl_auto ())
 =
   let (x, y) = par (left s) (right r) in
   x + y
@@ -34,12 +34,12 @@ let par3' (r s t : ref int) : ST int (fun p m -> exists v w u. m == (r |> v <*> 
 let ret (x:'a) () : ST 'a (fun p m -> m == emp /\ p x m) [] =
   x
 
-let set_to_2 (r : ref int) () : ST int (fun p m -> exists v. m == (r |> v) /\ p 1 (r |> 2)) [tosref r] =
+let set_to_2 (r : ref int) () : ST int (fun p m -> exists v. m == (r |> v) /\ p 1 (r |> 2)) [ii r] =
   r := 2;
   1
 
 (* Actually changing a reference *)
-let par_set (r:ref int) : ST int (fun p m -> exists v. m == r |> v /\ p 3 (r |> 2)) [tosref r] by (sl_auto ())
+let par_set (r:ref int) : ST int (fun p m -> exists v. m == r |> v /\ p 3 (r |> 2)) [ii r] by (sl_auto ())
 =
   let (x, y) = par (set_to_2 r) (ret 2) in
   x + y
@@ -62,20 +62,20 @@ let par_set (r:ref int) : ST int (fun p m -> exists v. m == r |> v /\ p 3 (r |> 
 (*   assert (dfst #int #(fun j -> int) (| 1, 2 |) == 1) *)
 (*       by (dump "1"; compute (); dump "2") *)
       
-let test_acq (r:ref int) (l:lock [tosref r] (fun _ -> True)) : ST int (fun p m -> m == emp /\ (forall v. p 3 (r |> v))) [tosref r]
+let test_acq (r:ref int) (l:lock [ii r] (fun _ -> True)) : ST int (fun p m -> m == emp /\ (forall v. p 3 (r |> v))) [ii r]
   by (sl_auto ())
     
   =
   acquire l;
   3
 
-let test_acq_rel (r:ref int) (l:lock [tosref r] (fun _ -> True)) : ST unit (fun p m -> m == emp /\ p () emp) [] by (sl_auto ())
+let test_acq_rel (r:ref int) (l:lock [ii r] (fun _ -> True)) : ST unit (fun p m -> m == emp /\ p () emp) [] by (sl_auto ())
   =
   acquire l;
   let v = !r in
   release l
 
-let set_and_ret (r:ref int) (l : lock [tosref r] (fun _ -> True)) (n : nat) () : ST int (fun p m -> m == emp /\ p n emp) [] by (sl_auto ()) =
+let set_and_ret (r:ref int) (l : lock [ii r] (fun _ -> True)) (n : nat) () : ST int (fun p m -> m == emp /\ p n emp) [] by (sl_auto ()) =
   acquire l;
   r := n;
   release l;
@@ -85,7 +85,7 @@ let set_and_ret (r:ref int) (l : lock [tosref r] (fun _ -> True)) (n : nat) () :
 
 (* Note: final heap is empty, it is the lock that owns `r` *)
 let test06 (r:ref int) : ST int (fun p m -> exists v. m == r |> v /\ p 3 emp) [] by (sl_auto ()) =
-  let l = mklock #(fun _ -> True) [tosref r]  in
+  let l = mklock #(fun _ -> True) [ii r]  in
   let (x, y) = par (set_and_ret r l 1) (set_and_ret r l 2) in
   x + y
 
@@ -94,12 +94,12 @@ let test07 () : ST int (fun p m -> m == emp /\ (forall r. p 3 (r |> 5))) [] by (
   3
   
 
-let test08 (r : ref int) : ST int (fun p m -> exists v. m == (r |> v) /\ (forall r'. p v (r |> v <*> r' |> v))) [tosref r] by (sl_auto ()) =
+let test08 (r : ref int) : ST int (fun p m -> exists v. m == (r |> v) /\ (forall r'. p v (r |> v <*> r' |> v))) [ii r] by (sl_auto ()) =
   let v = !r in
   let r' = alloc v in
   v
   
-let test09 (r : ref int) : ST int (fun p m -> exists v. m == (r |> v) /\ (forall r'. p v (r' |> v <*> r |> v))) [tosref r] by (sl_auto ()) =
+let test09 (r : ref int) : ST int (fun p m -> exists v. m == (r |> v) /\ (forall r'. p v (r' |> v <*> r |> v))) [ii r] by (sl_auto ()) =
   let v = !r in
   let r' = alloc v in
   v
@@ -119,7 +119,7 @@ let non_neg_inv (r:ref int) : memory -> Type0 =
 
 open FStar.Tactics
 
-let take_and_incr (r:ref int) (l : lock [tosref r] (fun m -> non_neg_inv r m)) : ST unit (fun p m -> m == emp /\ p () emp) [] by (sl_auto ()) =
+let take_and_incr (r:ref int) (l : lock [ii r] (fun m -> non_neg_inv r m)) : ST unit (fun p m -> m == emp /\ p () emp) [] by (sl_auto ()) =
   acquire l;
   r := !r + 1;
   release l
@@ -130,7 +130,7 @@ let take_and_incr (r:ref int) (l : lock [tosref r] (fun m -> non_neg_inv r m)) :
 
 let test12 () : ST unit (fun p m -> m == emp /\ p () emp) [] by (sl_auto ()) =
   let r = alloc 0 in
-  let l = mklock #(fun m -> non_neg_inv r m) [tosref r] in
+  let l = mklock #(fun m -> non_neg_inv r m) [ii r] in
   //let _ = par (fun () -> take_and_incr r l) (fun () -> take_and_incr r l) in
   //acquire l;
   //let v = !r in
@@ -140,7 +140,7 @@ let test12 () : ST unit (fun p m -> m == emp /\ p () emp) [] by (sl_auto ()) =
 
 let test13 () : ST unit (fun p m -> m == emp /\ p () emp) [] by (sl_auto ()) =
   let r = alloc 0 in
-  let l = mklock #(fun m -> non_neg_inv r m) [tosref r] in
+  let l = mklock #(fun m -> non_neg_inv r m) [ii r] in
   //let _ = par (fun () -> take_and_incr r l) (fun () -> take_and_incr r l) in
   acquire l;
   //let v = !r in
@@ -149,7 +149,7 @@ let test13 () : ST unit (fun p m -> m == emp /\ p () emp) [] by (sl_auto ()) =
 
 let test14 () : ST unit (fun p m -> m == emp /\ p () emp) [] by (sl_auto ()) =
   let r = alloc 0 in
-  let l = mklock #(fun m -> non_neg_inv r m) [tosref r] in
+  let l = mklock #(fun m -> non_neg_inv r m) [ii r] in
   let _ = par (fun () -> take_and_incr r l) (fun () -> take_and_incr r l) in
   acquire l;
   //let v = !r in
@@ -158,7 +158,7 @@ let test14 () : ST unit (fun p m -> m == emp /\ p () emp) [] by (sl_auto ()) =
 
 let test15 () : ST unit (fun p m -> m == emp /\ p () emp) [] by (sl_auto ()) =
   let r = alloc 0 in
-  let l = mklock #(fun m -> non_neg_inv r m) [tosref r] in
+  let l = mklock #(fun m -> non_neg_inv r m) [ii r] in
   let _ = par (fun () -> take_and_incr r l) (fun () -> take_and_incr r l) in
   acquire l;
   let v = !r in
@@ -167,7 +167,7 @@ let test15 () : ST unit (fun p m -> m == emp /\ p () emp) [] by (sl_auto ()) =
 
 let test16 () : ST unit (fun p m -> m == emp /\ p () emp) [] by (sl_auto ()) =
   let r = alloc 0 in
-  let l = mklock #(fun m -> non_neg_inv r m) [tosref r] in
+  let l = mklock #(fun m -> non_neg_inv r m) [ii r] in
   let _ = par (fun () -> take_and_incr r l) (fun () -> take_and_incr r l) in
   acquire l;
   let v = !r in
@@ -177,38 +177,38 @@ let test16 () : ST unit (fun p m -> m == emp /\ p () emp) [] by (sl_auto ()) =
 (* Double locks... hey, if it works for 1 and 2, it works for n *)
 
 let test17 (r s : ref int) : ST unit (fun p m -> exists v u. m == (r |> v <*> s |> u) /\ p () emp) [] by (sl_auto ()) =
-  let l = mklock #(fun m -> True) [tosref r; tosref s] in
+  let l = mklock #(fun m -> True) [ii r; ii s] in
   ()
 
 (* Same thing with the list backwards... should be robust *)
 let test17' (r s : ref int) : ST unit (fun p m -> exists v u. m == (r |> v <*> s |> u) /\ p () emp) [] by (sl_auto ()) =
-  let l = mklock #(fun m -> True) [tosref s; tosref r] in
+  let l = mklock #(fun m -> True) [ii s; ii r] in
   ()
 
 let test18 () : ST unit (fun p m -> m == emp /\ p () emp) [] by (sl_auto ()) =
   let r = alloc 0 in
   let s = alloc 1 in
-  let l = mklock #(fun m -> True) [tosref r; tosref s] in
+  let l = mklock #(fun m -> True) [ii r; ii s] in
   ()
 
 (* Coupled references *)
 let test19 () : ST unit (fun p m -> m == emp /\ p () emp) [] by (sl_auto ()) =
   let r = alloc 1 in
   let s = alloc 1 in
-  let l = mklock #(fun m -> exists v u. m == (r |> u <*> s |> v) /\ v == u)  [tosref r; tosref s] in
+  let l = mklock #(fun m -> exists v u. m == (r |> u <*> s |> v) /\ v == u)  [ii r; ii s] in
   ()
   
 let test20 () : ST unit (fun p m -> m == emp /\ (forall m'. p () m')) [] by (sl_auto ()) =
   let r = alloc 1 in
   let s = alloc 1 in
-  let l = mklock #(fun m -> exists v u. m == (r |> u <*> s |> v) /\ v == u)  [tosref r; tosref s] in
+  let l = mklock #(fun m -> exists v u. m == (r |> u <*> s |> v) /\ v == u)  [ii r; ii s] in
   acquire l;
   ()
 
 let test21 () : ST unit (fun p m -> m == emp /\ (forall m'. p () m')) [] by (sl_auto ()) =
   let r = alloc 1 in
   let s = alloc 1 in
-  let l = mklock #(fun m -> exists v u. m == (r |> u <*> s |> v) /\ v == u)  [tosref r; tosref s] in
+  let l = mklock #(fun m -> exists v u. m == (r |> u <*> s |> v) /\ v == u)  [ii r; ii s] in
   acquire l;
   let v = !r in
   let u = !s in
@@ -217,8 +217,7 @@ let test21 () : ST unit (fun p m -> m == emp /\ (forall m'. p () m')) [] by (sl_
 let test22 () : ST unit (fun p m -> m == emp /\ (forall m'. p () m')) [] by (sl_auto ()) =
   let r = alloc 1 in
   let s = alloc 1 in
-  let l = mklock #(fun m -> exists v u. mem_eq (m == (r |> u <*> s |> v)) /\ v == u)  [tosref r; tosref s] in
-  //let l = mklock #(fun m -> exists v u. m == (r |> u <*> s |> v) /\ v == u)  [tosref r; tosref s] in
+  let l = mklock #(fun m -> exists v u. mem_eq (m == (r |> u <*> s |> v)) /\ v == u)  [ii r; ii s] in
   acquire l;
   let v = !r in
   let u = !s in
@@ -230,7 +229,7 @@ assume val kinda_havoc : unit -> ST unit (fun p m -> m == emp /\ p () emp) []
 let test23 () : ST unit (fun p m -> m == emp /\ (forall m'. p () m')) [] by (sl_auto ()) =
   let r = alloc 1 in
   let s = alloc 1 in
-  let l = mklock #(fun m -> exists v u. mem_eq (m == (r |> u <*> s |> v)) /\ v == u)  [tosref r; tosref s] in
+  let l = mklock #(fun m -> exists v u. mem_eq (m == (r |> u <*> s |> v)) /\ v == u)  [ii r; ii s] in
   kinda_havoc ();
   acquire l;
   let v = !r in
