examples/csl/SL.ExamplesAuto.fst
@@ -5,11 +5,7 @@ open SL.AutoTactic
 
 let swap_wp (r1 r2:ref int) = fun p m -> exists x y. m == (r1 |> x <*> r2 |> y) /\ p () (r1 |> y <*> r2 |> x)
 
-(* #set-options "--tactic_trace_d 2 --debug SL.ExamplesAuto" *)
-
-//#set-options "--tactic_trace"
-
-let swap (r1 r2:ref int) : ST unit (swap_wp r1 r2) [tosref r1; tosref r2] by (sl_auto ())
+let swap (r1 r2:ref int) : ST unit (swap_wp r1 r2) [ii r1; ii r2] by (sl_auto ())
   = let x = !r1 in
     let y = !r2 in
     r1 := y;
@@ -18,26 +14,26 @@ let swap (r1 r2:ref int) : ST unit (swap_wp r1 r2) [tosref r1; tosref r2] by (sl
 let rotate_wp (r1 r2 r3:ref int)
   = fun p m -> exists x y z. m == (r1 |> x <*> r2 |> y <*> r3 |> z) /\ p () (r1 |> z <*> r2 |> x <*> r3 |> y)
 
-let rotate (r1 r2 r3:ref int) : ST unit (rotate_wp r1 r2 r3) [tosref r1; tosref r2; tosref r3] by (sl_auto ())
+let rotate (r1 r2 r3:ref int) : ST unit (rotate_wp r1 r2 r3) [ii r1; ii r2; ii r3] by (sl_auto ())
   = swap r2 r3;
     swap r1 r2
 
-let test (r1 r2:ref int) : ST int (fun p m -> exists x y. m == (r1 |> x <*> r2 |> y) /\ p x m) [tosref r1; tosref r2] by (sl_auto ())
+let test (r1 r2:ref int) : ST int (fun p m -> exists x y. m == (r1 |> x <*> r2 |> y) /\ p x m) [ii r1; ii r2] by (sl_auto ())
   = !r1
 
 (*
  * two commands
  *)
-let write_read (r1 r2:ref int) : ST int (fun p m -> exists x y. m == (r1 |> x <*> r2 |> y) /\ p y (r1 |> 2 <*> r2 |> y)) [tosref r1; tosref r2] by (sl_auto ())
+let write_read (r1 r2:ref int) : ST int (fun p m -> exists x y. m == (r1 |> x <*> r2 |> y) /\ p y (r1 |> 2 <*> r2 |> y)) [ii r1; ii r2] by (sl_auto ())
   = r1 := 2;
     !r2
 
-let read_write (r1 r2:ref int) : ST unit (fun p m -> exists x y. m == (r1 |> x <*> r2 |> y) /\ p () (r1 |> x <*> r2 |> x)) [tosref r1; tosref r2] by (sl_auto ())
+let read_write (r1 r2:ref int) : ST unit (fun p m -> exists x y. m == (r1 |> x <*> r2 |> y) /\ p () (r1 |> x <*> r2 |> x)) [ii r1; ii r2] by (sl_auto ())
   = let x = !r1 in
     r2 := x
 
 let cond_test (r:ref int) (b:bool) : ST unit (fun p m -> exists x. m == r |> x /\ ((b   ==> p () (r |> 1)) /\
-                                                                      (~ b ==> p () (r |> 2)))) [tosref r]
+                                                                      (~ b ==> p () (r |> 2)))) [ii r]
   by (sl_auto ())
 
   = if b then r := 1 else r := 2
@@ -45,7 +41,7 @@ let cond_test (r:ref int) (b:bool) : ST unit (fun p m -> exists x. m == r |> x /
 let rotate_left_or_right (r1 r2 r3:ref int) (b:bool)
   : ST unit (fun p m -> exists x y z. m == (r1 |> x <*> r2 |> y <*> r3 |> z) /\
                               ((b   ==> p () (r1 |> z <*> r2 |> x <*> r3 |> y)) /\
- 			      (~ b ==> p () (r1 |> y <*> r2 |> z <*> r3 |> x)))) [tosref r1; tosref r2; tosref r3]
+                               (~ b ==> p () (r1 |> y <*> r2 |> z <*> r3 |> x)))) [ii r1; ii r2; ii r3]
   by (sl_auto ())
 
   = if b then rotate r1 r2 r3 else rotate r3 r2 r1
